filter,unionをTableに移動した。

theorems/Tables.v
@@ -2,6 +2,8 @@ Require Import String.
 Require Import FMapWeakList.
 Require Import FMapInterface.
 Require Import FMapFacts.
+
+Require Import Util.
 Require Import Dec.
 
 Module Table := FMapWeakList.Make StrDec.
@@ -137,4 +139,111 @@ unfold Table.In,Table.Raw.PX.In in |- *.
 unfold Table.MapsTo in H.
 exists T.
 tauto.
+Qed.
+
+Definition union {A : Type} (tsubst1 tsubst2 : table A) :=
+  Table.fold (fun key e m => Table.add key e m) tsubst1 tsubst2.
+
+Definition filter {A : Type} {P : string -> Prop} (dec : forall x, {P x} + {~ P x}) (tsubst : table A) :=
+  TableProp.filter
+    (fun key _ => if dec key then true else false)
+    tsubst.
+
+Lemma union_iff: forall A x (T : A) (X Y : table A),
+  Table.MapsTo x T (union X Y) <->
+  Table.MapsTo x T X \/ (~ Table.In x X /\ Table.MapsTo x T Y).
+Proof.
+intros.
+unfold union in |- *.
+pattern X,
+ (Table.fold
+    (fun (key : Table.key) (e : A) (m : Table.t A) => Table.add key e m) X Y)
+ in |- *.
+apply TableProp.fold_rec_bis; intros.
+ apply Extensionality_Table in H.
+ rewrite <- H in |- *.
+ tauto.
+
+ split; intros; auto.
+  right.
+  split; auto.
+  intro.
+  apply TableWF.empty_in_iff in H0.
+  contradiction.
+
+  decompose [or and] H; auto.
+  inversion H0.
+
+ split; intros.
+  apply TableWF.add_mapsto_iff in H2.
+  decompose [or and] H2.
+   left.
+   rewrite H4, H5 in |- *.
+   apply <- TableWF.add_mapsto_iff.
+   tauto.
+
+   apply H1 in H5.
+   decompose [or and] H5.
+    left.
+    apply <- TableWF.add_mapsto_iff.
+    tauto.
+
+    right.
+    split; auto.
+    Contrapositive H6.
+    apply TableWF.add_in_iff in H3.
+    decompose [or] H3; auto.
+    contradiction.
+
+  decompose [or and] H2.
+   apply TableWF.add_mapsto_iff in H3.
+   decompose [or and] H3.
+    rewrite H5, H6 in |- *.
+    apply <- TableWF.add_mapsto_iff.
+    tauto.
+
+    apply <- TableWF.add_mapsto_iff.
+    tauto.
+
+   apply <- TableWF.add_mapsto_iff.
+   right.
+   split.
+    Contrapositive H4.
+    apply <- TableWF.add_in_iff.
+    tauto.
+
+    apply H1.
+    right.
+    split; auto.
+    Contrapositive H4.
+    apply <- TableWF.add_in_iff.
+    tauto.
+Qed.
+
+Lemma filter_iff : forall A x P (dec : forall x, {P x} + {~ P x}) (T : A) (m : table A),
+  Table.MapsTo x T (filter dec m) <->
+  Table.MapsTo x T m /\ (P x).
+Proof.
+unfold filter in |- *.
+split; intros.
+ apply TableProp.filter_iff in H.
+  unfold Morphisms.Morphism,Morphisms.respectful in |- *.
+  intros.
+  rewrite H0 in |- *.
+  reflexivity.
+
+  decompose [and] H.
+  split; auto.
+  destruct (dec x); auto.
+  discriminate.
+
+ apply <- TableProp.filter_iff.
+  decompose [and] H.
+  split; auto.
+  destruct (dec x); auto.
+
+  unfold Morphisms.Morphism, Morphisms.respectful in |- *.
+  intros.
+  rewrite H0 in |- *.
+  reflexivity.
 Qed.
